day7.thy
@@ -4,9 +4,19 @@ theory day7
   imports Main "HOL.Code_Numeral" string_utils list_natural_utils natural_utils list_utils
 begin
 
-text "This is a solution to the puzzle for day 6"
+text "This is a solution to the puzzle for day 7"
 
 subsection "Input parsing"
+
+text "Input parsing for today was a pain in the butt. If I had a language with powerful and easy to
+use string manipulations then this would be easy. Unfortunately I do not. So some of the string functions
+have been added for dealing with today's input. The input is still just a line-by-line thing, but it's
+presented in natural language. Fortunately it's quite predictable though."
+
+text "The bag\\_desc function takes one line of the input in the form of a list of tokens.
+A token is just one word from the input, where a word is defined such that you can tokenise the text
+simply by splitting on spaces. bag\\_desc figures out the name of the bag that this line
+describes, and then returns the token list for the subbag descriptions"
 
 primrec bag_desc :: "string \<Rightarrow> (string list) \<Rightarrow> (string * (string list))"
   where
@@ -17,6 +27,9 @@ primrec bag_desc :: "string \<Rightarrow> (string list) \<Rightarrow> (string * 
       else
         bag_desc (parsed @ '' '' @ t) toks
     )"
+
+text "sub\\_bags\\_parse takes the tokens that bag\\_desc didn't parse, and then produces a list of sub bag information.
+Each sub bag is a pair with a number (the number of bags of this type contained in the outer bag) and a name"
 
 fun sub_bags_parse :: "(natural * string) list \<Rightarrow> (natural * string) \<Rightarrow> string list \<Rightarrow> (natural * string) list"
   where
@@ -39,6 +52,9 @@ fun sub_bags_parse :: "(natural * string) list \<Rightarrow> (natural * string) 
     )
 )"
 
+text "Parsing a line of text is done by combining the two functions above, this is the parse\\_line
+function. parse\\_all returns a list of all bags in an input text"
+
 definition parse_line :: "string \<Rightarrow> (string * ((natural * string) list))"
   where "parse_line line = (let t = split CHR '' '' line in
     let (bd, sub_bags) = bag_desc '''' t in
@@ -49,7 +65,12 @@ definition parse_all where "parse_all s = map parse_line (split CHR ''\<newline>
 
 subsection "Solution Algorithm"
 
+text "The task concerns calculating some information about the shiny gold bag specifically. In part 1 we need
+to know how many different types of bag could hold a shiny gold bag at an arbitrary depth."
+
 definition p1col where "p1col = ''shiny gold''"
+
+text "First I define a function for getting information about a particular bag"
 
 primrec get_bag_info where
   "get_bag_info [] bag_col = undefined"
@@ -57,13 +78,20 @@ primrec get_bag_info where
   (if fst bag1_def = bag_col then snd bag1_def else get_bag_info bag_defs bag_col)
   "
 
+text "Then a function for getting all of the names of bags that we know about"
+
 definition all_bag_names where "all_bag_names bag_defs = map fst bag_defs"
+
+text "can\\_hold tells us what bags another bag can hold \\_directly\\_"
 
 definition can_hold where "can_hold bag_defs bag_col =
   (let names = all_bag_names bag_defs in
     filter (\<lambda> name . contains bag_col (map snd (get_bag_info bag_defs name))) names
   )
 "
+
+text "can\\_hold\\_rec tells us what bags another bag can hold \\_recursively\\_. To make sure that this function
+always terminates, I implemented a recursion limit."
 
 fun can_hold_rec :: "natural \<Rightarrow> (string \<times> (natural \<times> string) list) list \<Rightarrow> string list \<Rightarrow> string list" where
 "can_hold_rec limit bag_defs bag_cols = (if limit = 0 then undefined else  (let new_list =
@@ -73,8 +101,14 @@ fun can_hold_rec :: "natural \<Rightarrow> (string \<times> (natural \<times> st
 ))
 "
 
+text "part 1 is now simply the number of bags in can\\_hold\\_rec for the shiny gold bag"
+
 definition part1 :: "string \<Rightarrow> natural"
   where "part1 s = (natural_len (can_hold_rec 99 (parse_all s) [p1col])) - 1"
+
+text "part 2 is actually a bit simpler than part 1. it's faster than part1 given the data structure
+that I came up with for this task. It involves determining how many bags should end up inside the shiny
+gold bag. num\\_held calculates one more than this number"
 
 fun num_held :: "natural \<Rightarrow> _"
   where "num_held limit bag_defs bag_col = 
