day8.thy
@@ -1,0 +1,98 @@
+section "Solution to Day 8 of AoC 2020"
+
+theory day8
+  imports Main "HOL.Code_Numeral" string_utils list_natural_utils natural_utils list_utils
+begin
+
+text "This is a solution to the puzzle for day 8"
+
+subsection "Input parsing"
+
+datatype instr =
+  Nop
+  |Acc integer
+  |Jmp integer
+
+type_synonym program = "instr list"
+
+definition parse_instr
+  where "parse_instr s = (
+    case hd s of
+      CHR ''n'' \<Rightarrow> Nop
+      |CHR ''j'' \<Rightarrow> Jmp (str_to_int (drop 4 s))
+      |CHR ''a'' \<Rightarrow> Acc (str_to_int (drop 4 s))
+  )"
+
+lemma "parse_instr ''acc +7'' = Acc 7"
+  by eval
+
+lemma "parse_instr ''jmp -4'' = Jmp (- 4)"
+  by eval
+
+definition parse_program :: "string \<Rightarrow> program"
+  where "parse_program p = map parse_instr (split CHR ''\<newline>'' (trim p))"
+
+subsection "Solution Algorithm"
+
+definition exec_instr :: "instr \<Rightarrow> integer \<Rightarrow> integer \<times> integer"
+  where "exec_instr instr acc = (
+    case instr of
+      Nop \<Rightarrow> (acc, 1)
+      | Acc n \<Rightarrow> (acc + n, 1)
+      | Jmp n \<Rightarrow> (acc, n)
+  )"
+
+definition replace
+  where "replace n l new = (take_natural n l) @ [new] @ (drop (n + 1) l)"
+
+fun exec_program_until_loop :: "natural \<Rightarrow> _"
+  where
+    "exec_program_until_loop limit p flags acc pc = (
+    if limit = 0 then undefined else (
+      if nth pc flags then
+        acc
+      else
+        (let (new_acc, pc_change) = (exec_instr (nth pc p) acc) in
+          let new_flags = replace pc flags True in
+          exec_program_until_loop (limit - 1) p new_flags new_acc (natural_of_integer ((integer_of_natural pc) + pc_change))
+        )
+      )
+    )
+  "
+
+definition find_loop
+  where "find_loop p = (let flags = map (\<lambda> a . False) p in
+    exec_program_until_loop 9999 p flags 0 0
+  )"
+
+definition part1 :: "string \<Rightarrow> integer"
+  where "part1 s = find_loop (parse_program (trim s))"
+
+definition part2 :: "string \<Rightarrow> natural"
+  where "part2 s = 0"
+
+subsection "Testing"
+
+definition example_input::string where "example_input = ''
+nop +0
+acc +1
+jmp +4
+acc +3
+jmp -3
+acc -99
+acc +1
+jmp -4
+acc +6
+''"
+
+lemma "part1 example_input = 5"
+  by eval
+
+lemma "part2 example_input = 0"
+  by eval
+
+(* TODO remember to export part2 once complete *)
+
+export_code "part1" in Haskell module_name Solution
+
+end
