Makefile
@@ -1,5 +1,5 @@
 
-all_days=day1 day2 day3 day4 day5 day6 day7
+all_days=day1 day2 day3 day4 day5 day6 day7 day8
 
 default: test_all
 
@@ -7,12 +7,14 @@ export/AOC2020.%/code/export1/Solution.hs: %.thy
 	isabelle export -d . -x'*:**' AOC2020
 	sed -i -e 's/module Solution(\(.*\)Natural\(.*\)) where {/module Solution(\1 Natural(Nat) \2) where {/' export/AOC2020.*/code/export1/Solution.hs
 	sed -i -e 's/module Solution(\(.*\)Char\(.*\)) where {/module Solution(\1 Char(Char) \2) where {/' export/AOC2020.*/code/export1/Solution.hs
+	find export/AOC2020.*/code/export1/ -name Solution.hs -exec bash -c 'grep "module Solution.*Natural" {} > /dev/null || sed -i -e "s/module Solution(/module Solution ( Natural(Nat),/" {}' ';'
 
 .PRECIOUS:: export/AOC2020.%/code/export1/Solution.hs
 
 objs/runner_%.o: runner.hs export/AOC2020.%/code/export1/Solution.hs
 	mkdir -p objs
-	ghc -c $< -o $@ -i$(dir $(word 2,$^)) -ohi objs/runner_$*.hi -cpp '-DDAY_NUMBER=("$*")' '-DTODAYS_INPUT=("inputs/$*.txt")' "-D$$(grep '^part2 ::' $(word 2,$^) > /dev/null && echo 'RUN_PART2' || echo 'SKIP_PART2')"
+	ghc -c $< -o $@ -i$(dir $(word 2,$^)) -ohi objs/runner_$*.hi -cpp '-DDAY_NUMBER=("$*")' '-DTODAYS_INPUT=("inputs/$*.txt")' "-D$$(grep '^part2 ::' $(word 2,$^) > /dev/null && echo 'RUN_PART2' || echo 'SKIP_PART2')" "-DINTEGER_SUPPORT=0$$(grep 'part[1-2] *:: *\[Char\] *-> *Integer;' $(word 2,$^) > /dev/null && echo '1')" "-DP1INTEGER=0$$(grep 'part1 *:: *\[Char\] *-> *Integer;' $(word 2,$^) > /dev/null && echo '1')" "-DP2INTEGER=0$$(grep 'part2 *:: *\[Char\] *-> *Integer;' $(word 2,$^) > /dev/null && echo '1')"
+
     
 objs/%.o: export/AOC2020.%/code/export1/Solution.hs
 	mkdir -p objs
